Weidenbach_Book/CDCL_Two_Watched_Literals_Implementation.thy
@@ -1,0 +1,10 @@
+(*  Title: CDCL with Two Watched Literals
+    Author: Mathias Fleury <mathias.fleury@mpi-inf.mpg.de>
+*)
+
+theory CDCL_Two_Watched_Literals_Implementation
+imports CDCL_Two_Watched_Literals
+begin
+
+
+end
